Remove extraneous ctx duplicates from substs

src/named/IntensionalModel.v
@@ -14,8 +14,6 @@ with subst : ctx -> Type :=
 But: can't have ctx in type of subst
  *)
 
-Require Import JMeq.
-
 (*
 Definition eq_conv : forall A, A -> forall B, B -> Prop.
   intros A a B b.
@@ -25,26 +23,31 @@ Defined. *)
 
 Section Inner.
   
-  Context (subst_n : nat -> (forall A : Type, A -> Prop) -> Type).
+  Context (subst_n : nat -> forall A : Type, A -> Type).
   Fixpoint ctx_n (n : nat) : Type :=
     match n with
     | 0 => unit
-    | S n0 => {c : ctx_n n0 & subst_n n0 (JMeq c) -> Type}
+    | S n0 => {c : ctx_n n0 & subst_n n0 c -> Type}
     end.
 
 End Inner.
 
-Fixpoint subst_n (n : nat) (P : forall A : Type, A -> Prop) : Type :=
+Definition conv {A B} (Heq : A = B) : A -> B :=
+  match Heq in _ = B return A -> B with eq_refl => @id _ end.
+
+Fixpoint subst_n (n : nat) A (a : A) {struct n} : Type :=
   let ctx_n := ctx_n subst_n in
   match n with
   | 0 => unit
-  | S n' => {c : ctx_n (S n') & {_ : P (ctx_n (S n')) c & {s : subst_n n' (JMeq (projT1 c)) & projT2 c s}}}
+  | S n' =>
+      {Heq : A = ctx_n (S n') &
+               let c := conv Heq a in
+               {s : subst_n n' (projT1 c) & projT2 c s}}
   end.
 
-Definition ctx := { n & ctx_n subst_n n}.
-Definition subst (c : ctx) := subst_n (projT1 c) (JMeq (projT2 c)).
 
-    
+Definition ctx := { n & ctx_n subst_n n}.
+Definition subst (c : ctx) := subst_n (projT1 c) (projT2 c).
 
 Definition ctx_nil : ctx := existT _ 0 tt.
 Definition ctx_cons : forall (c : ctx), (subst c -> Type) -> ctx :=
@@ -94,13 +97,18 @@ Definition subst_cons : forall (c : ctx) (s : subst c) (A : subst c -> Type) (e 
     let (n, c) as s return (forall (s0 : subst s) (A : subst s -> Type),
                         A s0 -> subst (ctx_cons s A)) :=
       c
-    in (fun s A e => existT _ (existT _ c A) (existT _ JMeq_refl (existT _ s e))).
+    in fun s _ e => {#eq_refl; s; e #}.
 
-(*TODO: either go back to eq_conv, prove this from UIP,
-  or find a way to discharge it
- *)
-Axiom JMeq_UIP_refl
-  : forall (U : Type) (x : U) (p : JMeq x x), p = JMeq_refl.
+Require Import Eqdep.
+Import EqdepTheory.
+(*
+Lemma conv_id {A} (p : A = A) x : conv p x = x.
+Proof.
+  unfold conv.
+  replace p with (eq_refl A); auto.
+  apply UIP.
+Qed.
+*)
 
 Lemma subst_ind {P : forall {c : ctx}, subst c -> Prop}
   (P_nil : P subst_nil)
@@ -117,26 +125,44 @@ Proof.
   }
   {
     destruct c as [c A].
-    destruct s as [c' [Heq [s e]]].
-    destruct c'.
+    destruct s as [Heq [s e]].
+
     simpl in *.
-    pose proof (Heq' := Heq).
-    apply JMeq_eq in Heq'.
-    inversion Heq'.
-    subst.
-    clear H1.
-    assert (A = T) by (apply Eqdep.EqdepTheory.inj_pair2 in Heq'; auto).
-    subst.
-    clear Heq'.
-    rewrite (JMeq_UIP_refl Heq).
-    clear Heq.
-    
-    specialize (P_cons (existT _ n x) s).
+    revert Heq s e.
+    refine (Streicher_K _ _ _ _).
+    simpl.
+    intros.
+    change {# eq_refl; s; e #} with (subst_cons {# n; c #} s A e).
+    change {# S n; c; A #} with (ctx_cons {# n; c #} A).
     eapply P_cons.
     eapply IHn.
   }
 Qed.
 
+Definition eq_rect_r
+  : forall (A : Type) (x : A) (P : A -> Type), P x -> forall y : A, y = x -> P y :=
+  fun (A : Type) (x : A) P (H : P x) (y : A) (H0 : y = x) =>
+    eq_rect x (fun y0 : A => P y0) H y (eq_sym H0).
+
+Definition Type_Streicher_K_on_ := 
+fun (U : Type) (x : U) (P : x = x -> Type) => P eq_refl -> forall p : x = x, P p.
+
+Definition Type_UIP_refl_on__Streicher_K_on
+  : forall (U : Type) (x : U) (P : x = x -> Type), UIP_refl_on_ U x -> Type_Streicher_K_on_ P
+  := 
+  fun (U : Type) (x : U) P (UIP_refl : UIP_refl_on_ U x) (H : P eq_refl) (p : x = x) =>
+    eq_rect_r P H (UIP_refl p).
+
+Definition Type_Streicher_K_ := fun U : Type => forall (x : U) (P : x = x -> Type), Type_Streicher_K_on_ P.
+
+Definition Type_UIP_refl__Streicher_K
+  : forall U : Type, UIP_refl_ U -> Type_Streicher_K_ U
+  := 
+  fun (U : Type) (UIP_refl : UIP_refl_ U) (x : U) (P : x = x -> Type) =>
+    Type_UIP_refl_on__Streicher_K_on P (UIP_refl x).
+
+Definition Type_Streicher_K : forall (U : Type) (x : U) (P : x = x -> Type), P eq_refl -> forall p : x = x, P p :=
+  fun U : Type => Type_UIP_refl__Streicher_K (UIP_refl U).
 
 (* TODO: make a version with a good definition for computing*)
 Lemma subst_rect {P : forall {c : ctx}, subst c -> Type}
@@ -154,21 +180,15 @@ Proof.
   }
   {
     destruct c as [c A].
-    destruct s as [c' [Heq [s e]]].
-    destruct c'.
+    destruct s as [Heq [s e]].
+
     simpl in *.
-    pose proof (Heq' := Heq).
-    apply JMeq_eq in Heq'.
-    inversion Heq'.
-    subst.
-    clear H1.
-    assert (A = T) by (apply Eqdep.EqdepTheory.inj_pair2 in Heq'; auto).
-    subst.
-    clear Heq'.
-    rewrite (JMeq_UIP_refl Heq).
-    clear Heq.
-    
-    specialize (P_cons (existT _ n x) s).
+    revert Heq s e.
+    refine (Type_Streicher_K _ _).
+    simpl.
+    intros.
+    change {# eq_refl; s; e #} with (subst_cons {# n; c #} s A e).
+    change {# S n; c; A #} with (ctx_cons {# n; c #} A).
     eapply P_cons.
     eapply IHn.
   }
@@ -190,10 +210,10 @@ Notation "|# x1 ; .. ; xn #|" :=
   (ctx_cons .. (ctx_cons ctx_nil x1) .. xn)
     (format "'|#'  '[hv' x1 ;  .. ;  xn ']'  '#|'").
 
-
+(*
 Require Import Program.Basics.
 
-Local Open Scope program_scope.
+Local Open Scope program_scope.*)
 
 (*TODO: return an option?*)
 Definition ctx_tl' n : ctx_n subst_n n -> ctx_n subst_n (pred n) :=
@@ -222,52 +242,38 @@ Definition ctx_hd : forall (c : ctx), sort (ctx_tl c) :=
   fun c =>
   let (n, c') as c' return sort (ctx_tl c') := c in ctx_hd' _ _.
 
+(*TODO: check that this computes*)
 Definition subst_tl' n
   : forall (c : ctx_n subst_n n),
     msubst {# n; c #} (ctx_tl {# n; c #}).
   refine (
-    match n as n
-          return forall (c : ctx_n subst_n n),
-        msubst {# n; c #} (ctx_tl {# n; c #})
-    with
-    | 0 => fun c => id
-    | S _ => fun c => _
-    end).
+      match n as n
+            return forall (c : ctx_n subst_n n),
+          msubst {# n; c #} (ctx_tl {# n; c #})
+      with
+      | 0 => fun _ _ => tt
+      | S n0 =>
+          fun c =>
+            let (c, A) as c return msubst {# S n0; c #} (ctx_tl {# S n0; c #})
+              := c in  _
+      end).
   simpl in c.
-  refine
-    (let (c, A) as c return msubst {# S n0; c #} (ctx_tl {# S n0; c #})
-       := c in  _).
-  simpl in *.
   intro s.
-  unfold subst in *.
-  clear c0.
-  simpl in *.
+  simpl.
   destruct s.
-  destruct x.
-  destruct s.
-  assert (c = x).
-  {
-    refine (match x0 in JMeq {# c; A #} {# x; T #}
-                  return c = x with
-            | _ => _
-            end).
-    destruct x0.
-    inversion x0.
-  in
-  refine (let (n,c') as c return msubst c (ctx_tl c) := c in _)
-  
-  refine (projT2 _).
-  {
-    simpl.
-    e
-  refine (fun c => _).
-  refine (let (n,c') as c return msubst c (ctx_tl c) := c in _).
+  revert x s.
+  refine (Type_Streicher_K _ _).
+  simpl.
+  eapply projT1.
+Defined.
   
 Definition subst_tl : forall (c : ctx), msubst c (ctx_tl c).
   refine (fun c => _).
   refine (let (n,c') as c return msubst c (ctx_tl c) := c in _).
   refine (fun s => _).
-  simpl.
+  eapply subst_tl'; eauto.
+  TODO: universe issues
+Defined.
 
 
 (* TODO: make a version with a good definition for computing*)
